crypto_examples/ntt_rec3.dfy
@@ -1,0 +1,87 @@
+include "ntt_rec2.dfy"
+
+module ntt_recs3 {
+    import opened Seq
+    import opened Power
+    import opened Power2
+    import opened DivMod
+    import opened Mul
+    import opened pows_of_2
+    import opened omegas
+    import opened rindex
+    import opened ntt_recs2
+    import opened ntt_rec
+
+   function method ntt_rec3_base(ghost a: seq<seq<elem>>, len: pow2_t, ghost idxs: seq<seq<index_t>>): (ys: seq<seq<elem>>)
+        requires ntt_chunk_indicies_inv(a, idxs, len);
+        requires len.full == 1 && len.exp == 0;
+        ensures ntt_chunks_eval_inv(a, idxs, ys, len);
+    {
+        nth_root_lemma();
+        var ys := seq(N, i requires 0 <= i < N => [Ar()[i]]);
+        assert ntt_chunks_eval_inv(a, idxs, ys, len) by {
+            forall ki: nat | ki < |a| 
+                ensures poly_eval_all_points(a[ki], ys[ki], len)
+            {
+                ntt_indicies_inv_consequence0(a[ki], idxs[ki], len, ki);
+                ntt_rec_base_case(a[ki], len);
+            }
+        }
+        ys
+    }
+
+    function method ntt_rec3(ghost a: seq<seq<elem>>, len: pow2_t, ghost idxs: seq<seq<index_t>>): (ys: seq<seq<elem>>)
+        requires ntt_chunk_indicies_inv(a, idxs, len);
+        requires 1 <= len.full;
+        requires 0 <= len.exp <= L;
+        ensures ntt_chunks_eval_inv(a, idxs, ys, len);
+        decreases len.exp;
+    {
+        pow2_basics(len);
+        if len.full == 1 then 
+            ntt_rec3_base(a, len, idxs)
+        else
+            var len' := pow2_half(len);
+            var count := pow2_div(pow2(L), len).full;
+            var count' := pow2_div(pow2(L), len').full;
+            assume count' == pow2_div(pow2(L), len).full * 2;
+
+            ghost var a' := seq(count', i  requires 0 <= i < count' => 
+                if i % 2 == 0 then even_indexed_terms(a[i/2], len)
+                else odd_indexed_terms(a[i/2], len));
+
+            ghost var idxs' := seq(count', i  requires 0 <= i < count' => 
+                if i % 2 == 0 then even_indexed_indices(idxs[i/2], len)
+                else odd_indexed_indices(idxs[i/2], len));
+
+            assert ntt_chunk_indicies_inv(a', idxs', len') by {
+                forall i | 0 <= i < count'
+                    ensures ntt_indicies_inv(a'[i], idxs'[i], len', i);
+                {
+                    var ki := i/2;
+
+                    var ai: seq<elem> := a[i/2];
+                    var idx := idxs[i/2];
+        
+                    assert ntt_indicies_inv(a[ki], idxs[ki], len, ki);
+    
+                    if i % 2 == 0 {
+                        ghost var a_e := even_indexed_terms(ai, len);
+                        ghost var idx_e := even_indexed_indices(idx, len);
+                        even_indexed_indices_reorder(ai, idx, len, a_e, idx_e, ki);
+                    } else {
+                        ghost var a_o := odd_indexed_terms(ai, len);
+                        ghost var idx_o := odd_indexed_indices(idx, len);
+                        odd_indexed_indices_reorder(ai, idx, len, a_o, idx_o, ki);
+                    }
+                }
+            }
+            var ys' := ntt_rec3(a', len', idxs');
+
+            ntt_rec2_chunk_combine_feasible(a, a', len, count, count', idxs, idxs', ys');
+
+            var ys := seq(count, i  requires 0 <= i < count => 
+                ntt_rec2_combine(a[i], a'[2 * i], a'[2 * i + 1], len, idxs[i], ys'[i * 2], ys'[i * 2 + 1], i));
+            ys
+    }
+}
